fixed wrong git commands

src/dvspec/dafny/att_spec_proofs/core_proofs.dfy
@@ -99,13 +99,21 @@ module Core_Proofs
                         ==> && var tempSet := dvn.globally_signed_attestations - { a };
                             && !is_slashable_attestation_data_in_set_of_attestations(tempSet, a.data);
     }
+    predicate is_slashable_attestation_data_eth_spec(data_1: AttestationData, data_2: AttestationData)
+    {
+        || (data_1 != data_2 && data_1.target.epoch == data_2.target.epoch)
+        || (data_1.source.epoch < data_2.source.epoch && data_2.target.epoch < data_1.target.epoch)
+    }
 
-    lemma lemma_4_1(dvn: DVState, a: Attestation, a': Attestation, hn: BLSPubkey, hn': BLSPubkey)
+
+    lemma lemma_4_1_a(dvn: DVState, a: Attestation, a': Attestation, hn: BLSPubkey, hn': BLSPubkey)
     requires |dvn.all_nodes| > 0
     requires pred_4_1_b(dvn)
     requires pred_4_1_c(dvn)
     requires pred_4_1_f_a(dvn)
     requires inv42(dvn)
+    requires pred_4_1_g_a(dvn)
+    requires pred_4_1_g_b(dvn)
     requires hn in dvn.honest_nodes_states.Keys 
     requires hn' in dvn.honest_nodes_states.Keys
     requires a in dvn.honest_nodes_states[hn].bn.attestations_submitted
@@ -113,18 +121,8 @@ module Core_Proofs
     requires a.data.slot < a'.data.slot 
     requires isConditionForSafetyTrue(dvn.consensus_on_attestation_data[a.data.slot])
     requires isConditionForSafetyTrue(dvn.consensus_on_attestation_data[a'.data.slot])
-    // ensures   
-    //         var sdba := SlashingDBAttestation(
-    //                         source_epoch := a.data.source.epoch,
-    //                         target_epoch := a.data.target.epoch,
-    //                         signing_root := None
-    //                 );   
-    //         var sdba' := SlashingDBAttestation(
-    //                         source_epoch := a'.data.source.epoch,
-    //                         target_epoch := a'.data.target.epoch,
-    //                         signing_root := None
-    //                 );                       
-    //         !is_slashable_attestation_pair(sdba, sdba')
+    ensures && !is_slashable_attestation_data_eth_spec(a.data, a'.data)
+            && !is_slashable_attestation_data_eth_spec(a'.data, a.data)
     {
         var hna, att_share :|
                 && hna in dvn.honest_nodes_states.Keys 
@@ -179,7 +177,134 @@ module Core_Proofs
             
         var m: BLSPubkey :| m in honest_nodes && m in h_nodes_a && m in h_nodes_a';  
 
-        assert m in  consa.honest_nodes_validity_functions.Keys;      
+        assert m in  consa.honest_nodes_validity_functions.Keys; 
+        assert m in  consa'.honest_nodes_validity_functions.Keys; 
+
+        var vpa: AttestationData -> bool :| 
+            vpa in consa.honest_nodes_validity_functions[m] && vpa(consa.decided_value.safe_get()); 
+
+        var vpa': AttestationData -> bool :| 
+            vpa' in consa'.honest_nodes_validity_functions[m] && vpa'(consa'.decided_value.safe_get()); 
+
+        var attestation_duty', attestation_slashing_db' :|
+                vpa' == (ad: AttestationData) => consensus_is_valid_attestation_data(attestation_slashing_db', ad, attestation_duty');   
+
+        assert consa.decided_value.isPresent();  
+
+        var decided_a_data := consa.decided_value.safe_get();
+        var sdba := SlashingDBAttestation(
+                                        source_epoch := decided_a_data.source.epoch,
+                                        target_epoch := decided_a_data.target.epoch,
+                                        signing_root := Some(hash_tree_root(decided_a_data)));
+        assert sdba in attestation_slashing_db';     
+
+        assert !is_slashable_attestation_data(attestation_slashing_db', a'.data);
+
+        var sdba' := SlashingDBAttestation(
+                                        source_epoch := a'.data.source.epoch,
+                                        target_epoch := a'.data.target.epoch,
+                                        signing_root := None);        
+
+        lemma_is_slashable_attestation_data(attestation_slashing_db', a'.data, sdba', sdba);
+        assert !is_slashable_attestation_data_eth_spec(a.data, a'.data);
+        assert !is_slashable_attestation_data_eth_spec(a'.data, a.data);
+        
+    }    
+
+    lemma lemma_4_1_b(dvn: DVState, a: Attestation, a': Attestation, hn: BLSPubkey, hn': BLSPubkey)
+    requires |dvn.all_nodes| > 0
+    requires pred_4_1_b(dvn)
+    requires pred_4_1_c(dvn)
+    requires pred_4_1_f_a(dvn)
+    requires inv42(dvn)
+    requires pred_4_1_g_a(dvn)
+    requires pred_4_1_g_b(dvn)
+    requires hn in dvn.honest_nodes_states.Keys 
+    requires hn' in dvn.honest_nodes_states.Keys
+    requires a in dvn.honest_nodes_states[hn].bn.attestations_submitted
+    requires a' in dvn.honest_nodes_states[hn'].bn.attestations_submitted
+    requires a.data.slot == a'.data.slot 
+    requires isConditionForSafetyTrue(dvn.consensus_on_attestation_data[a.data.slot])
+    requires isConditionForSafetyTrue(dvn.consensus_on_attestation_data[a'.data.slot])
+    ensures && !is_slashable_attestation_data_eth_spec(a.data, a'.data)
+            && !is_slashable_attestation_data_eth_spec(a'.data, a.data)
+    {
+        var hna, att_share :|
+                && hna in dvn.honest_nodes_states.Keys 
+                && att_share in dvn.att_network.allMessagesSent
+                && att_share.data == a.data
+                && var fork_version := bn_get_fork_version(compute_start_slot_at_epoch(att_share.data.target.epoch));
+                && var attestation_signing_root := compute_attestation_signing_root(att_share.data, fork_version);
+                && verify_bls_siganture(attestation_signing_root, att_share.signature, hna);     
+
+        var hna', att_share' :|
+                && hna' in dvn.honest_nodes_states.Keys 
+                && att_share' in dvn.att_network.allMessagesSent
+                && att_share'.data == a'.data
+                && var fork_version := bn_get_fork_version(compute_start_slot_at_epoch(att_share'.data.target.epoch));
+                && var attestation_signing_root := compute_attestation_signing_root(att_share'.data, fork_version);
+                && verify_bls_siganture(attestation_signing_root, att_share'.signature, hna');  
+
+        var cons := dvn.consensus_on_attestation_data[a.data.slot];                 
+
+        assert
+                && cons.decided_value.isPresent()
+                && cons.decided_value.safe_get() == att_share.data
+                && cons.decided_value.safe_get() == att_share'.data;     
+
+        assert a.data == a'.data;  
+
+        assert !is_slashable_attestation_data_eth_spec(a.data, a'.data);
+        assert !is_slashable_attestation_data_eth_spec(a'.data, a.data);        
+    }      
+
+    lemma lemma_4_1_general(dvn: DVState, a: Attestation, a': Attestation, hn: BLSPubkey, hn': BLSPubkey)
+    requires |dvn.all_nodes| > 0
+    requires pred_4_1_b(dvn)
+    requires pred_4_1_c(dvn)
+    requires pred_4_1_f_a(dvn)
+    requires inv42(dvn)
+    requires pred_4_1_g_a(dvn)
+    requires pred_4_1_g_b(dvn)
+    requires hn in dvn.honest_nodes_states.Keys 
+    requires hn' in dvn.honest_nodes_states.Keys
+    requires a in dvn.honest_nodes_states[hn].bn.attestations_submitted
+    requires a' in dvn.honest_nodes_states[hn'].bn.attestations_submitted
+    requires isConditionForSafetyTrue(dvn.consensus_on_attestation_data[a.data.slot])
+    requires isConditionForSafetyTrue(dvn.consensus_on_attestation_data[a'.data.slot])
+    ensures && !is_slashable_attestation_data_eth_spec(a.data, a'.data)
+            && !is_slashable_attestation_data_eth_spec(a'.data, a.data)   
+    {
+        if a.data.slot == a'.data.slot 
+        {
+            lemma_4_1_b(dvn, a, a', hn, hn');
+        }
+        else if a.data.slot < a'.data.slot 
+        {
+            lemma_4_1_a(dvn, a, a', hn, hn');
+        }
+        else {
+            lemma_4_1_a(dvn, a', a, hn', hn);
+        }
+    } 
+
+    lemma lemma_is_slashable_attestation_data(
+        att_slashing_db: set<SlashingDBAttestation>, 
+        ad: AttestationData,
+        sdba: SlashingDBAttestation,
+        sdba': SlashingDBAttestation
+
+    )
+    requires !is_slashable_attestation_data(att_slashing_db, ad)
+    requires sdba' in att_slashing_db
+    requires sdba.source_epoch == ad.source.epoch 
+    requires sdba.target_epoch == ad.target.epoch 
+    ensures !is_slashable_attestation_pair(sdba, sdba')
+    ensures !is_slashable_attestation_pair(sdba', sdba)
+    {
+
+    }
+            
                     
         // TODO: Prove 4 g - i with lemma_decided_value_is_not_slashable_with_slashing_db_that_constructed_vp
         // and invariants 43--45.
